backend/Allocproof.v
@@ -2653,29 +2653,8 @@ Proof.
   eapply plus_left. constructor.
   destruct (transf_function_inv _ _ FUN).
   rewrite <- COMP. rewrite <- type_of_call_translated.
-  intros G. specialize (NO_CROSS_PTR G).
-  unfold loc_result.
-  { intros l Hl.
-    (* assert (Htype_list: Val.has_type_list rs ## args (sig_args sg)). *)
-    (* { inv WTI. rewrite <- H10. *)
-    (*   clear -WTRS. eapply wt_regset_list. eauto. } *)
-    clear -RES NO_CROSS_PTR Hl.
-    unfold loc_result in RES.
-    destruct (proj_sig_res sg) eqn:Hsg;
-      subst; simpl in *; try intuition; subst.
-    inv RES; auto; try contradiction.
-    inv RES; auto; try contradiction.
-    destruct (Archi.ptr64); simpl in *; try intuition; subst.
-    inv RES; auto; try contradiction.
-    inv RES; auto; try contradiction.
-    destruct (ls (R R11)); simpl in *; auto.
-    inv RES; auto; try contradiction.
-    destruct (ls (R R11)); simpl in *; try contradiction.
-    destruct (ls (R R10)); simpl in *; auto; try contradiction.
-    inv RES; auto; try contradiction.
-    inv RES; auto; try contradiction.
-    inv RES; auto; try contradiction.
-  }
+  intros G. specialize (NO_CROSS_PTR G). clear -RES NO_CROSS_PTR.
+  now inv RES.
   eexact A. traceEq.
   econstructor; eauto.
   apply wt_regset_assign; auto. rewrite WTRES0; auto.
